restoring proofs and connecting to PRFSetHash

steel/Veritas.Steel.PRFSetHash.fst
@@ -19,77 +19,107 @@ module VF = Veritas.Formats
 module MSH = Veritas.MultiSetHash
 module HA = Veritas.Steel.HashAccumulator
 
-let prf_set_hash = HA.state
+noeq
+type prf_set_hash = {
+  ha_state : HA.state;
+  serialization_buf: a:A.array U8.t{A.length a == 184 }
+}
+
+let prf_set_hash_vprop (s:prf_set_hash)
+  : vprop
+  = A.varray s.ha_state `star`
+    A.varray s.serialization_buf
 
 let prf_set_hash_sl (s:prf_set_hash)
   : slprop u#1
-  = A.is_array s
+  = hp_of (prf_set_hash_vprop s)
+
+let prf_set_hash_repr
+  : Type0
+  = (HA.hash_value_t & A.contents U8.t 184)
+
+let hash_value_of (p:prf_set_hash_repr) = fst p
 
 let prf_set_hash_sel (r:prf_set_hash)
-  : selector (HA.hash_value_t) (prf_set_hash_sl r)
-  = A.array_sel r
+  : GTot (selector prf_set_hash_repr (prf_set_hash_sl r))
+  = sel_of (prf_set_hash_vprop r)
 
+//how to prove these?
+let intro_set_hash_inv #o (s:prf_set_hash)
+  : SteelGhost unit o
+    (A.varray s.ha_state `star` A.varray s.serialization_buf)
+    (fun _ -> prf_set_hash_inv s)
+    (requires fun _ -> True)
+    (ensures fun h0 _ h1 ->
+      v_hash s h1 == A.asel s.ha_state h0)
+  = AT.sladmit()
+let elim_set_hash_inv #o (s:prf_set_hash)
+  : SteelGhost unit o
+    (prf_set_hash_inv s)
+    (fun _ -> A.varray s.ha_state `star` A.varray s.serialization_buf)
+    (requires fun _ -> True)
+    (ensures fun h0 _ h1 ->
+      v_hash s h0 == A.asel s.ha_state h1)
+  = AT.sladmit()
+
+//#push-options "--query_stats"
 let create () =
   let x = HA.create_in () in
-  AT.change_equal_slprop (A.varray _)
-                         (prf_set_hash_inv _);
-  AT.return x
+  let buf = A.malloc 0uy 184ul in
+  let res = {
+    ha_state = x;
+    serialization_buf = buf
+  } in
+  AT.change_equal_slprop (A.varray x `star` A.varray buf)
+                         (A.varray res.ha_state `star` A.varray res.serialization_buf);
+  intro_set_hash_inv res;
+  AT.return res
 
 let free (p:prf_set_hash)
-  = AT.change_equal_slprop (prf_set_hash_inv _)
-                           (A.varray _);
-    HA.free p
+  = elim_set_hash_inv p;
+    HA.free p.ha_state;
+    A.free p.serialization_buf
 
-let update_hash_value (ha:HA.hash_value_t)
-                      (r:T.record)
-                      (t:T.timestamp)
-                      (tid:T.thread_id)
-  : GTot HA.hash_value_t
-  = let b = VF.serialize_stamped_record_spec (VFT.({ sr_record = r; sr_timestamp = t; sr_thread_id = tid})) in
-    let h = HA.hash_value b in
-    HA.aggregate_hash_value ha h
-
-#push-options "--query_stats"
-let prf_update_hash' (p:prf_set_hash)
+//#push-options "--query_stats"
+let prf_update_hash' (p:HA.state)
                      (r:T.record)
                      (t:T.timestamp)
                      (tid:T.thread_id)
+                     (buf:A.array U8.t)
   : Steel unit
-    (A.varray p)
-    (fun _ -> A.varray p)
-    (requires fun _ -> True)
+    (A.varray p `star` A.varray buf)
+    (fun _ -> A.varray p `star` A.varray buf)
+    (requires fun _ ->
+      A.length p == 32 /\
+      A.length buf == 184)
     (ensures fun h0 _ h1 ->
-      A.asel p h1 == update_hash_value (A.asel p h0) r t tid)
+      A.asel p h1 == VM.update_hash_value (A.asel p h0) r t tid)
   =  let h0 = AT.get () in
      let sr = (VFT.({ sr_record = r; sr_timestamp = t; sr_thread_id = tid})) in
-     let tmp = A.malloc 0uy 184ul in
-     let len = VF.serialize_stamped_record tmp sr in
+     let len = VF.serialize_stamped_record buf sr in
      let h1 = AT.get () in
-     HA.add p tmp len;
-     A.free tmp;
+     HA.add p buf len;
      AT.slassert (A.varray p);
      let h2 = AT.get () in
      assert (A.asel p h2 ==
              HA.aggregate_hash_value (A.asel p h1)
                                      (HA.hash_value
-                                       (Seq.slice (A.asel tmp h1) 0 (U32.v len))));
-     assert (Seq.slice (A.asel tmp h1) 0 (U32.v len) ==
+                                       (Seq.slice (A.asel buf h1) 0 (U32.v len))));
+     assert (Seq.slice (A.asel buf h1) 0 (U32.v len) ==
              VF.serialize_stamped_record_spec sr);
      assert (A.asel p h2 ==
              HA.aggregate_hash_value
                (A.asel p h1)
                (HA.hash_value (VF.serialize_stamped_record_spec sr)));
      assert_spinoff (A.asel p h2 ==
-                     update_hash_value (A.asel p h1) r t tid)
+                     VM.update_hash_value (A.asel p h1) r t tid)
 
 let prf_update_hash p r t tid =
-  AT.change_equal_slprop (prf_set_hash_inv p)
-                         (A.varray p);
-  prf_update_hash' p r t tid;
-  AT.change_equal_slprop (A.varray p)
-                         (prf_set_hash_inv p)
+  elim_set_hash_inv p;
+  prf_update_hash' p.ha_state r t tid p.serialization_buf;
+  intro_set_hash_inv p
 
-let prf_read_hash' (p:prf_set_hash) (out:A.array U8.t)
+let prf_read_hash' (p:HA.state) (out:A.array U8.t)
   : Steel unit
     (A.varray p `star` A.varray out)
     (fun _ -> A.varray p `star` A.varray out)
@@ -101,11 +131,9 @@ let prf_read_hash' (p:prf_set_hash) (out:A.array U8.t)
   = HA.get p out
 
 let prf_read_hash (p:prf_set_hash) (out:A.array U8.t)
-  = AT.change_equal_slprop (prf_set_hash_inv p)
-                           (A.varray p);
-    prf_read_hash' p out;
-    AT.change_equal_slprop (A.varray p)
-                           (prf_set_hash_inv p)
+  = elim_set_hash_inv p;
+    prf_read_hash' p.ha_state out;
+    intro_set_hash_inv p
 
 let prf_hash_agg (a0 a1:A.array U8.t)
   : Steel unit
