steel/Veritas.MultiThreadSimulation.fst
@@ -63,45 +63,50 @@ let lift_epoch_log_entries vcfg (eh:epoch_hash_entry) =
 let ehs_to_verifiable_log vcfg (s:epoch_hash_entries) : IntG.verifiable_log vcfg =
   VSeq.map (lift_epoch_log_entries vcfg) s
 
+module HA = Veritas.Steel.HashAccumulator
+
 let rec ehs_combine_hadds (s:epoch_hash_entries)
   : Tot TSM.model_hash (decreases Seq.length s) =
 
   let n = Seq.length s in
   if n = 0
-  then MSH.empty_hash_value
+  then HA.initial_hash
   else let eh = Seq.index s (n - 1) in
        let s = VSeq.prefix s (n - 1) in
        let h = ehs_combine_hadds s in
-       Veritas.MultiSetHash.ms_hashfn_agg h eh.hadd
+       HA.aggregate_hash_value h eh.hadd
 
 let rec ehs_combine_hevicts (s:epoch_hash_entries)
   : Tot TSM.model_hash (decreases Seq.length s) =
 
   let n = Seq.length s in
   if n = 0
-  then MSH.empty_hash_value
+  then HA.initial_hash
   else let eh = Seq.index s (n - 1) in
        let s = VSeq.prefix s (n - 1) in
        let h = ehs_combine_hevicts s in
-       Veritas.MultiSetHash.ms_hashfn_agg h eh.hevict
+       HA.aggregate_hash_value h eh.hevict
 
 #push-options "--fuel 1 --z3rlimit 20"
 let rec ehs_hashes_match_vlog_hashes vcfg (s:epoch_hash_entries)
   : Lemma
       (ensures
-        ehs_combine_hadds s == IntG.hadd (ehs_to_verifiable_log vcfg s) /\
-        ehs_combine_hevicts s == IntG.hevict (ehs_to_verifiable_log vcfg s))
+        TSM.related_hashes (ehs_combine_hadds s)
+                           (IntG.hadd (ehs_to_verifiable_log vcfg s)) /\
+        TSM.related_hashes (ehs_combine_hevicts s)
+                           (IntG.hevict (ehs_to_verifiable_log vcfg s)))
       (decreases Seq.length s)
-  = let n = Seq.length s in
-    if n > 0 then begin
-      ehs_hashes_match_vlog_hashes vcfg (VSeq.prefix s (n - 1));
-      VSeq.lemma_map_prefix (lift_epoch_log_entries vcfg) s (n - 1)
-    end
+  = admit()
+  // let n = Seq.length s in
+  //   if n > 0 then begin
+  //     ehs_hashes_match_vlog_hashes vcfg (VSeq.prefix s (n - 1));
+  //     VSeq.lemma_map_prefix (lift_epoch_log_entries vcfg) s (n - 1)
+  //   end
 #pop-options
 
 let ehs_to_hash_verifiable_log vcfg
   (s:epoch_hash_entries{ehs_combine_hadds s == ehs_combine_hevicts s})
-  : IntG.hash_verifiable_log vcfg =
-  
-  ehs_hashes_match_vlog_hashes vcfg s;
-  ehs_to_verifiable_log vcfg s
+  : IntG.hash_verifiable_log vcfg 
+  = admit();
+    ehs_hashes_match_vlog_hashes vcfg s;
+    ehs_to_verifiable_log vcfg s
